very monotonic boilerplate (up to example)

src/ExprImp.v
@@ -1,9 +1,5 @@
-Set Universe Polymorphism.
-Unset Universe Minimization ToSet.
-(* TODO: should we do this? *)
-Set Primitive Projections.
-Unset Printing Primitive Projection Parameters.
-Set Printing Projections.
+Ltac typeof x := match type of x with ?T => T end.
+Notation "'typeof!' x" := (ltac:(let T := typeof x in exact T)) (at level 10).
 
 Require compiler.Common.
 
@@ -35,200 +31,214 @@ Record ImpParameters :=
     store : mword -> mword -> mem -> option mem;
   }.
 
-Section Imp.
-  Context {p : ImpParameters}.
-  (* RecordImport p (* COQBUG(https://github.com/coq/coq/issues/7808) *) *)
-  Local Notation mword := p.(mword).
-  Local Notation mword_nonzero := p.(mword_nonzero).
-  Local Notation varname := p.(varname).
-  Local Notation funname := p.(funname).
-  Local Notation actname := p.(actname).
-  Local Notation bopname := p.(bopname).
-  Local Notation varmap := p.(varmap).
-  Local Notation mem := p.(mem).
-  Local Definition varmap_operations_ : Common.Map _ _ _ := p.(varmap_operations). Global Existing Instance varmap_operations_.
-  Local Notation interp_binop := p.(interp_binop).
-  Local Notation load := p.(load).
-  Local Notation store := p.(store).
+Module Imp_.
+  Section Imp_.
+    Context {p : ImpParameters}.
+    (* RecordImport p (* COQBUG(https://github.com/coq/coq/issues/7808) *) *)
+    Local Notation mword := p.(mword).
+    Local Notation mword_nonzero := p.(mword_nonzero).
+    Local Notation varname := p.(varname).
+    Local Notation funname := p.(funname).
+    Local Notation actname := p.(actname).
+    Local Notation bopname := p.(bopname).
+    Local Notation varmap := p.(varmap).
+    Local Notation mem := p.(mem).
+    Local Definition varmap_operations_ : Common.Map _ _ _ := p.(varmap_operations). Global Existing Instance varmap_operations_.
+    Local Notation interp_binop := p.(interp_binop).
+    Local Notation load := p.(load).
+    Local Notation store := p.(store).
+    Local Inductive expr  : Type :=
+    | ELit(v: mword)
+    | EVar(x: varname)
+    | EOp(op: bopname) (e1 e2: expr).
 
-  Record ImpInterface :=
-    {
-      expr : Type;
-      ELit : mword -> expr;
-      EVar : varname -> expr;
-      EOp : bopname -> expr -> expr -> expr;
+    Local Inductive stmt :=
+    | SLoad(x: varname) (addr: expr)
+    | SStore(addr val: expr)
+    | SSet(x: varname)(e: expr)
+    | SIf(cond: expr)(bThen bElse: stmt)
+    | SWhile(cond: expr)(body: stmt)
+    | SSeq(s1 s2: stmt)
+    | SSkip
+    | SCall(binds: list varname)(f: funname)(args: list expr)
+    | SIO(binds: list varname)(io : actname)(args: list expr).
 
-      stmt : Type;
+    Section cont.
+      Context {T : Type}.
+      Local Inductive cont : Type :=
+      | CSuspended(_:T)
+      | CSeq(s1:cont) (s2: stmt)
+      | CStack(st: varmap)(c: cont)(binds rets: list varname).
+    End cont. Global Arguments cont : clear implicits.
 
-      SLoad : varname -> expr -> stmt;
-      SStore : expr -> expr -> stmt;
-      SSet : varname -> expr -> stmt;
-      SIf : expr -> stmt -> stmt -> stmt;
-      SWhile : expr -> stmt -> stmt;
-      SSeq : stmt -> stmt -> stmt;
-      SSkip : stmt;
-      SCall : list varname -> funname -> list expr -> stmt;
-      SIO : list varname -> actname -> list expr -> stmt;
+    Local Definition ioact : Type := (list varname * actname * list mword).
+    Local Definition ioret : Type := (list varname * list mword).
 
-      cont : Type -> Type;
-      CSuspended : forall T, T -> cont T;
-      CSeq : forall T, cont T -> stmt -> cont T;
-      CStack : forall T, varmap -> cont T -> list varname -> list varname -> cont T;
+    Local Fixpoint interp_expr st e : option mword :=
+      match e with
+      | ELit v => Some v
+      | EVar x => Common.get st x
+      | EOp op e1 e2 =>
+        bind_Some v1 <- interp_expr st e1;
+          bind_Some v2 <- interp_expr st e2;
+          Some (interp_binop op v1 v2)
+      end.
 
-      ioact : Type;
-      ioret : Type;
-
-      interp_expr : forall (st: varmap)(e: expr), option (mword);
-      interp_stmt : forall (lookupFunction : funname -> option (list varname * list varname * stmt))(f: nat)(st: varmap)(m: mem)(s: stmt),       option (varmap*mem*option(cont ioact));
-      interp_cont : forall (lookupFunction : funname -> option (list varname * list varname * stmt))(f: nat)(st: varmap)(m: mem)(s: cont ioret), option (varmap*mem*option(cont ioact));
-    }.
-
-  Local Inductive _expr :=
-  | _ELit(v: mword)
-  | _EVar(x: varname)
-  | _EOp(op: bopname) (e1 e2: _expr).
-
-  Local Inductive _stmt :=
-  | _SLoad(x: varname) (addr: _expr)
-  | _SStore(addr val: _expr)
-  | _SSet(x: varname)(e: _expr)
-  | _SIf(cond: _expr)(bThen bElse: _stmt)
-  | _SWhile(cond: _expr)(body: _stmt)
-  | _SSeq(s1 s2: _stmt)
-  | _SSkip
-  | _SCall(binds: list varname)(f: funname)(args: list _expr)
-  | _SIO(binds: list varname)(io : actname)(args: list _expr).
-
-  Local Fixpoint _interp_expr(st: varmap)(e: _expr): option (mword) :=
-    match e with
-    | _ELit v => Some v
-    | _EVar x => Common.get st x
-    | _EOp op e1 e2 =>
-        bind_Some v1 <- _interp_expr st e1;
-        bind_Some v2 <- _interp_expr st e2;
-        Some (interp_binop op v1 v2)
-    end.
-
-  Section cont.
-    Context {T : Type}.
-    Local Inductive _cont : Type :=
-    | _CSuspended(_:T)
-    | _CSeq(s1:_cont) (s2: _stmt)
-    | _CStack(st: varmap)(c: _cont)(binds rets: list varname).
-  End cont. Arguments _cont : clear implicits.
-
-  Local Definition _ioact : Type := (list varname * actname * list mword).
-  Local Definition _ioret : Type := (list varname * list mword).
-  
-  Section WithFunctions.
-    Context (lookupFunction : funname -> option (list varname * list varname * _stmt)).
-    Local Fixpoint _interp_stmt(f: nat)(st: varmap)(m: mem)(s: _stmt): option (varmap*mem*option(_cont _ioact)) :=
-      match f with
-      | 0 => None (* out of fuel *)
-      | S f => match s with
-        | _SLoad x a =>
-            bind_Some a <- _interp_expr st a;
-            bind_Some v <- load a m;
-            Some (Common.put st x v, m, None)
-        | _SStore a v =>
-            bind_Some a <- _interp_expr st a;
-            bind_Some v <- _interp_expr st v;
-            bind_Some m <- store a v m;
-            Some (st, m, None)
-        | _SSet x e =>
-            bind_Some v <- _interp_expr st e;
-            Some (Common.put st x v, m, None)
-        | _SIf cond bThen bElse =>
-            bind_Some v <- _interp_expr st cond;
-            _interp_stmt f st m (if mword_nonzero v then bThen else bElse)
-        | _SWhile cond body =>
-            bind_Some v <- _interp_expr st cond;
-            if mword_nonzero v
-            then
-              bind_Some (st, m, c) <- _interp_stmt f st m body;
+    Section WithFunctions.
+      Context (lookupFunction : funname -> option (list varname * list varname * stmt)).
+      Local Fixpoint interp_stmt(f: nat)(st: varmap)(m: mem)(s: stmt): option (varmap*mem*option(cont ioact)) :=
+        match f with
+        | 0 => None (* out of fuel *)
+        | S f => match s with
+          | SLoad x a =>
+              bind_Some a <- interp_expr st a;
+              bind_Some v <- load a m;
+              Some (Common.put st x v, m, None)
+          | SStore a v =>
+              bind_Some a <- interp_expr st a;
+              bind_Some v <- interp_expr st v;
+              bind_Some m <- store a v m;
+              Some (st, m, None)
+          | SSet x e =>
+              bind_Some v <- interp_expr st e;
+              Some (Common.put st x v, m, None)
+          | SIf cond bThen bElse =>
+              bind_Some v <- interp_expr st cond;
+              interp_stmt f st m (if mword_nonzero v then bThen else bElse)
+          | SWhile cond body =>
+              bind_Some v <- interp_expr st cond;
+              if mword_nonzero v
+              then
+                bind_Some (st, m, c) <- interp_stmt f st m body;
+                match c with
+                | Some c => Some (st, m, Some (CSeq c (SWhile cond body)))
+                | None => interp_stmt f st m (SWhile cond body)
+                end
+              else Some (st, m, None)
+          | SSeq s1 s2 =>
+              bind_Some (st, m, c) <- interp_stmt f st m s1;
               match c with
-              | Some c => Some (st, m, Some (_CSeq c (_SWhile cond body)))
-              | None => _interp_stmt f st m (_SWhile cond body)
+              | Some c => Some (st, m, Some (CSeq c s2))
+              | None => interp_stmt f st m s2
               end
-            else Some (st, m, None)
-        | _SSeq s1 s2 =>
-            bind_Some (st, m, c) <- _interp_stmt f st m s1;
-            match c with
-            | Some c => Some (st, m, Some (_CSeq c s2))
-            | None => _interp_stmt f st m s2
-            end
-        | _SSkip => Some (st, m, None)
-        | _SCall binds fname args =>
-          bind_Some (params, rets, fbody) <- lookupFunction fname;
-          bind_Some argvs <- Common.option_all (List.map (_interp_expr st) args);
-          bind_Some st0 <- Common.putmany params argvs Common.empty;
-          bind_Some (st1, m', oc) <- _interp_stmt f st0 m fbody;
-          match oc with
-          | Some c => Some (st, m', Some (_CStack st1 c binds rets))
-          | None => 
-            bind_Some retvs <- Common.option_all (List.map (Common.get st1) rets);
-            bind_Some st' <- Common.putmany binds retvs st;
-            Some (st', m', None)
-          end
-        | _SIO binds ionum args =>
-          bind_Some argvs <- Common.option_all (List.map (_interp_expr st) args);
-          Some (st, m, Some (_CSuspended (binds, ionum, argvs)))
-        end
-      end.
-
-    Local Fixpoint _interp_cont(f: nat)(st: varmap)(m: mem)(s: _cont _ioret): option (varmap*mem*option(_cont _ioact)) :=
-      match f with
-      | 0 => None (* out of fuel *)
-      | S f => match s with
-        | _CSuspended (binds, retvs) =>
-            bind_Some st' <- Common.putmany binds retvs st;
-            Some (st', m, None)
-        | _CSeq c s2 =>
-            bind_Some (st, m, oc) <- _interp_cont f st m c;
+          | SSkip => Some (st, m, None)
+          | SCall binds fname args =>
+            bind_Some (params, rets, fbody) <- lookupFunction fname;
+            bind_Some argvs <- Common.option_all (List.map (interp_expr st) args);
+            bind_Some st0 <- Common.putmany params argvs Common.empty;
+            bind_Some (st1, m', oc) <- interp_stmt f st0 m fbody;
             match oc with
-            | Some c => Some (st, m, Some (_CSeq c s2))
-            | None => _interp_stmt f st m s2
+            | Some c => Some (st, m', Some (CStack st1 c binds rets))
+            | None => 
+              bind_Some retvs <- Common.option_all (List.map (Common.get st1) rets);
+              bind_Some st' <- Common.putmany binds retvs st;
+              Some (st', m', None)
             end
-        | _CStack stf cf binds rets =>
-          bind_Some (stf', m', oc) <- _interp_cont f stf m cf;
-          match oc with
-          | Some c => Some (st, m', Some (_CStack stf' c binds rets))
-          | None => 
-            bind_Some retvs <- Common.option_all (List.map (Common.get stf') rets);
-            bind_Some st' <- Common.putmany binds retvs st;
-            Some (st', m', None)
+          | SIO binds ionum args =>
+            bind_Some argvs <- Common.option_all (List.map (interp_expr st) args);
+            Some (st, m, Some (CSuspended (binds, ionum, argvs)))
           end
-        end
-      end.
-  End WithFunctions.
+        end.
 
-  Definition Imp : ImpInterface :=
-        {|
-          ELit := _ELit;
-          EVar := _EVar;
-          EOp := _EOp;
+      Local Fixpoint interp_cont(f: nat)(st: varmap)(m: mem)(s: cont ioret): option (varmap*mem*option(cont ioact)) :=
+        match f with
+        | 0 => None (* out of fuel *)
+        | S f => match s with
+          | CSuspended (binds, retvs) =>
+              bind_Some st' <- Common.putmany binds retvs st;
+              Some (st', m, None)
+          | CSeq c s2 =>
+              bind_Some (st, m, oc) <- interp_cont f st m c;
+              match oc with
+              | Some c => Some (st, m, Some (CSeq c s2))
+              | None => interp_stmt f st m s2
+              end
+          | CStack stf cf binds rets =>
+            bind_Some (stf', m', oc) <- interp_cont f stf m cf;
+            match oc with
+            | Some c => Some (st, m', Some (CStack stf' c binds rets))
+            | None => 
+              bind_Some retvs <- Common.option_all (List.map (Common.get stf') rets);
+              bind_Some st' <- Common.putmany binds retvs st;
+              Some (st', m', None)
+            end
+          end
+        end.
+    End WithFunctions.
+  End Imp_.
+  Global Arguments expr : clear implicits.
+  Global Arguments stmt : clear implicits.
+  Global Arguments cont : clear implicits.
+End Imp_.
 
-          SLoad := _SLoad;
-          SStore := _SStore;
-          SSet := _SSet;
-          SIf := _SIf;
-          SWhile := _SWhile;
-          SSeq := _SSeq;
-          SSkip := _SSkip;
-          SCall := _SCall;
-          SIO := _SIO;
+Record ImpInterface {p:ImpParameters} :=
+  {
+    expr : typeof! (@Imp_.expr p);
+    ELit : typeof! (@Imp_.ELit p);
+    EVar : typeof! (@Imp_.EVar p);
+    EOp : typeof! (@Imp_.EOp p);
+    expr_rect : typeof! (@Imp_.expr_rect p);
 
-          CSuspended := @_CSuspended;
-          CSeq := @_CSeq;
-          CStack := @_CStack;
+    stmt : typeof! (@Imp_.stmt p);
+    SLoad : typeof! (@Imp_.SLoad p);
+    SStore : typeof! (@Imp_.SStore p);
+    SSet : typeof! (@Imp_.SSet p);
+    SIf : typeof! (@Imp_.SIf p);
+    SWhile : typeof! (@Imp_.SWhile p);
+    SSeq : typeof! (@Imp_.SSeq p);
+    SSkip : typeof! (@Imp_.SSkip p);
+    SCall : typeof! (@Imp_.SCall p);
+    SIO : typeof! (@Imp_.SIO p);
+    stmt_rect : typeof! (@Imp_.stmt_rect p);
 
-          interp_expr := _interp_expr;
-          interp_stmt := _interp_stmt;
-          interp_cont := _interp_cont;
-        |}.
-End Imp.
-Arguments ImpInterface : clear implicits.
-Arguments Imp : clear implicits.
+    cont : typeof! (@Imp_.cont p);
+    CSuspended : typeof! (@Imp_.CSuspended p);
+    CSeq : typeof! (@Imp_.CSeq p);
+    CStack : typeof! (@Imp_.CStack p);
+    cont_rect : typeof! (@Imp_.cont_rect p);
+
+    ioact : typeof! (@Imp_.ioact p);
+    ioret : typeof! (@Imp_.ioret p);
+
+    interp_expr : typeof! (@Imp_.interp_expr p);
+    interp_stmt : typeof! (@Imp_.interp_stmt p);
+    interp_cont : typeof! (@Imp_.interp_cont p);
+  }.
+Global Arguments ImpInterface : clear implicits.
+
+Definition Imp (p : ImpParameters) : ImpInterface p :=
+  {|
+    expr := @Imp_.expr p;
+    ELit := @Imp_.ELit p;
+    EVar := @Imp_.EVar p;
+    EOp := @Imp_.EOp p;
+    expr_rect := @Imp_.expr_rect p;
+    
+    stmt := @Imp_.stmt p;
+    SLoad := @Imp_.SLoad p;
+    SStore := @Imp_.SStore p;
+    SSet := @Imp_.SSet p;
+    SIf := @Imp_.SIf p;
+    SWhile := @Imp_.SWhile p;
+    SSeq := @Imp_.SSeq p;
+    SSkip := @Imp_.SSkip p;
+    SCall := @Imp_.SCall p;
+    SIO := @Imp_.SIO p;
+    stmt_rect := @Imp_.stmt_rect p;
+
+    cont := Imp_.cont p;
+    CSuspended := @Imp_.CSuspended p;
+    CSeq := @Imp_.CSeq p;
+    CStack := @Imp_.CStack p;
+    cont_rect := @Imp_.cont_rect p;
+    
+    ioact := @Imp_.ioact p;
+    ioret := @Imp_.ioret p;
+
+    interp_expr := @Imp_.interp_expr p;
+    interp_stmt := @Imp_.interp_stmt p;
+    interp_cont := @Imp_.interp_cont p;
+  |}.
 
 End Imp. (* TODO: file *)
 
@@ -312,34 +322,24 @@ Section ImpInversion.
   Local Notation interp_cont := Imp.(interp_cont).
   
   Lemma cont_uninhabited (T:Set) (_:T -> False) (X : cont T) : False. Proof. induction X; auto 2. Qed.
-  Fixpoint lift_cont {A B : Set} (P : A -> B -> Prop) (a : cont A) (b : cont B) {struct a} :=
-    match a, b with
-    | _CSuspended a, _CSuspended b =>
-      P a b
-    | _CSeq a sa, _CSeq b sb =>
-      lift_cont P a b /\ sa = sb
-    | _CStack sta a ba ra, _CStack stb b bb rb =>
-      (forall v, Common.get sta v = Common.get stb v) /\ lift_cont P a b /\ ba = bb /\ ra = rb
-    | _, _ => False
-    end.
 
   Fixpoint expr_size(e: expr): nat :=
     match e with
-    | _ELit _ => 8
-    | _EVar _ => 1
-    | _EOp op e1 e2 => S (S (expr_size e1 + expr_size e2))
+    | Imp_.ELit _ => 8
+    | Imp_.EVar _ => 1
+    | Imp_.EOp op e1 e2 => S (S (expr_size e1 + expr_size e2))
     end.
 
   Fixpoint stmt_size(s: stmt): nat :=
     match s with
-    | _SLoad x a => S (expr_size a)
-    | _SStore a v => S (expr_size a + expr_size v)
-    | _SSet x e => S (expr_size e)
-    | _SIf cond bThen bElse => S (expr_size cond + stmt_size bThen + stmt_size bElse)
-    | _SWhile cond body => S (expr_size cond + stmt_size body)
-    | _SSeq s1 s2 => S (stmt_size s1 + stmt_size s2)
-    | _SSkip => 1
-    | _SCall binds _ args | _SIO binds _ args =>
+    | Imp_.SLoad x a => S (expr_size a)
+    | Imp_.SStore a v => S (expr_size a + expr_size v)
+    | Imp_.SSet x e => S (expr_size e)
+    | Imp_.SIf cond bThen bElse => S (expr_size cond + stmt_size bThen + stmt_size bElse)
+    | Imp_.SWhile cond body => S (expr_size cond + stmt_size body)
+    | Imp_.SSeq s1 s2 => S (stmt_size s1 + stmt_size s2)
+    | Imp_.SSkip => 1
+    | Imp_.SCall binds _ args | Imp_.SIO binds _ args =>
                            S (length binds + length args + List.fold_right Nat.add O (List.map expr_size args))
     end.
 
@@ -351,14 +351,14 @@ Section ImpInversion.
     eauto 99.
 
   Lemma invert_interp_SLoad: forall env fuel initialSt initialM x e final,
-      interp_stmt env (S fuel) initialSt initialM (SLoad _ x e) = Some final ->
+      interp_stmt env (S fuel) initialSt initialM (Imp.(SLoad) x e) = Some final ->
       exists a v, interp_expr initialSt e = Some a /\
                   load a initialM = Some v /\
                   final = (put initialSt x v, initialM, None).
   Proof. inversion_lemma. Qed.
 
   Lemma invert_interp_SStore: forall env fuel initialSt initialM a v final,
-    interp_stmt env (S fuel) initialSt initialM (SStore _ a v) = Some final ->
+    interp_stmt env (S fuel) initialSt initialM (Imp.(SStore) a v) = Some final ->
     exists av vv finalM, interp_expr initialSt a = Some av /\
                          interp_expr initialSt v = Some vv /\
                          store av vv initialM = Some finalM /\
@@ -366,12 +366,12 @@ Section ImpInversion.
   Proof. inversion_lemma. Qed.
 
   Lemma invert_interp_SSet: forall env f st1 m1 p2 x e,
-    interp_stmt env (S f) st1 m1 (SSet _ x e) = Some p2 ->
+    interp_stmt env (S f) st1 m1 (Imp.(SSet) x e) = Some p2 ->
     exists v, interp_expr st1 e = Some v /\ p2 = (put st1 x v, m1, None).
   Proof. inversion_lemma. Qed.
 
   Lemma invert_interp_SIf: forall env f st1 m1 p2 cond bThen bElse,
-    interp_stmt env (S f) st1 m1 (SIf _ cond bThen bElse) = Some p2 ->
+    interp_stmt env (S f) st1 m1 (Imp.(SIf) cond bThen bElse) = Some p2 ->
     exists cv,
       interp_expr st1 cond = Some cv /\ 
       (mword_nonzero cv = true /\ interp_stmt env f st1 m1 bThen = Some p2 \/
@@ -379,30 +379,30 @@ Section ImpInversion.
   Proof. inversion_lemma. Qed.
 
   Lemma invert_interp_SSkip: forall env st1 m1 p2 f,
-    interp_stmt env (S f) st1 m1 (SSkip _) = Some p2 ->
+    interp_stmt env (S f) st1 m1 Imp.(SSkip) = Some p2 ->
     p2 = (st1, m1, None).
   Proof. inversion_lemma. Qed.
 
   Lemma invert_interp_SSeq: forall env st1 m1 p3 f s1 s2,
-    interp_stmt env (S f) st1 m1 (SSeq _ s1 s2) = Some p3 ->
+    interp_stmt env (S f) st1 m1 (Imp.(SSeq) s1 s2) = Some p3 ->
     exists st2 m2 oc, interp_stmt env f st1 m1 s1 = Some (st2, m2, oc) /\ (
         (oc = None /\ interp_stmt env f st2 m2 s2 = Some p3)
-     \/ (exists c, oc = Some c /\ p3 = (st2, m2, Some (CSeq _ _ c s2)))).
+     \/ (exists c, oc = Some c /\ p3 = (st2, m2, Some (Imp.(CSeq) _ c s2)))).
   Proof. inversion_lemma. Qed.
 
   Lemma invert_interp_SWhile: forall env st1 m1 p3 f cond body,
-    interp_stmt env (S f) st1 m1 (SWhile _ cond body) = Some p3 ->
+    interp_stmt env (S f) st1 m1 (Imp.(SWhile) cond body) = Some p3 ->
     exists cv,
       interp_expr st1 cond = Some cv /\
       (mword_nonzero cv = true /\
        (exists st2 m2 oc, interp_stmt env f st1 m1 body = Some (st2, m2, oc) /\ (
-              ( oc = None /\ interp_stmt env f st2 m2 (SWhile _ cond body) = Some p3)
-           \/ ( exists c, oc = Some c /\ p3 = (st2, m2, Some (CSeq _ _ c (SWhile _ cond body))))))
+              ( oc = None /\ interp_stmt env f st2 m2 (Imp.(SWhile) cond body) = Some p3)
+           \/ ( exists c, oc = Some c /\ p3 = (st2, m2, Some (Imp.(CSeq) _ c (Imp.(SWhile) cond body))))))
        \/ mword_nonzero cv = false /\ p3 = (st1, m1, None)).
   Proof. inversion_lemma. Qed.
 
   Lemma invert_interp_SCall : forall env st m1 p2 f binds fname args,
-    interp_stmt env (S f) st m1 (SCall _ binds fname args) = Some p2 ->
+    interp_stmt env (S f) st m1 (Imp.(SCall) binds fname args) = Some p2 ->
     exists params rets fbody argvs st0 st1 m' oc,
       env fname = Some (params, rets, fbody) /\
       option_all (map (interp_expr st) args) = Some argvs /\
@@ -414,13 +414,13 @@ Section ImpInversion.
          p2 = (st', m', None)
        ) \/
        ( exists c, oc = Some c /\
-         p2 = (st, m', Some (CStack _ _ st1 c binds rets)) ) ).
+         p2 = (st, m', Some (Imp.(CStack) _ st1 c binds rets)) ) ).
   Proof. inversion_lemma. Qed.
 
   Lemma invert_interp_SIO : forall env st m1 p2 f binds ioname args,
-    interp_stmt env (S f) st m1 (SIO _ binds ioname args) = Some p2 ->
-    exists argvs, option_all (map (Imp.interp_expr _ st) args) = Some argvs /\
-                  p2 = (st, m1, Some (CSuspended _ _ (binds, ioname, argvs))).
+    interp_stmt env (S f) st m1 (Imp.(SIO) binds ioname args) = Some p2 ->
+    exists argvs, option_all (map (interp_expr st) args) = Some argvs /\
+                  p2 = (st, m1, Some (Imp.(CSuspended) _ (binds, ioname, argvs))).
   Proof. inversion_lemma. Qed.
 End ImpInversion.
 
@@ -468,26 +468,26 @@ Section ImpVars.
   Local Notation interp_cont := Imp.(interp_cont).
 
   (* TODO: record ImpParametersOK *)
-  Context {mword_eq_dec : DecidableRel (@eq (Imp.varname p))}.
+  Context {mword_eq_dec : DecidableEq (Imp.varname p)}.
 
   (* Returns a list to make it obvious that it's a finite set. *)
   Fixpoint allVars_expr(e: expr): list varname :=
     match e with
-    | _ELit v => []
-    | _EVar x => [x]
-    | _EOp op e1 e2 => (allVars_expr e1) ++ (allVars_expr e2)
+    | Imp_.ELit v => []
+    | Imp_.EVar x => [x]
+    | Imp_.EOp op e1 e2 => (allVars_expr e1) ++ (allVars_expr e2)
     end.
 
   Fixpoint allVars_stmt(s: stmt): list varname := 
     match s with
-    | _SLoad v e => v :: allVars_expr e
-    | _SStore a e => (allVars_expr a) ++ (allVars_expr e)
-    | _SSet v e => v :: allVars_expr e
-    | _SIf c s1 s2 => (allVars_expr c) ++ (allVars_stmt s1) ++ (allVars_stmt s2)
-    | _SWhile c body => (allVars_expr c) ++ (allVars_stmt body)
-    | _SSeq s1 s2 => (allVars_stmt s1) ++ (allVars_stmt s2)
-    | _SSkip => []
-    | _SCall binds _ args | _SIO binds _ args => binds ++ List.fold_right (@List.app _) nil (List.map allVars_expr args)
+    | Imp_.SLoad v e => v :: allVars_expr e
+    | Imp_.SStore a e => (allVars_expr a) ++ (allVars_expr e)
+    | Imp_.SSet v e => v :: allVars_expr e
+    | Imp_.SIf c s1 s2 => (allVars_expr c) ++ (allVars_stmt s1) ++ (allVars_stmt s2)
+    | Imp_.SWhile c body => (allVars_expr c) ++ (allVars_stmt body)
+    | Imp_.SSeq s1 s2 => (allVars_stmt s1) ++ (allVars_stmt s2)
+    | Imp_.SSkip => []
+    | Imp_.SCall binds _ args | Imp_.SIO binds _ args => binds ++ List.fold_right (@List.app _) nil (List.map allVars_expr args)
     end.
 
   Context {set_varname: Type}.
@@ -497,14 +497,14 @@ Section ImpVars.
      The returned set might be too big, but is guaranteed to include all modified vars. *)
   Fixpoint modVars(s: stmt): set_varname := 
     match s with
-    | _SLoad v _ => singleton_set v
-    | _SStore _ _ => empty_set
-    | _SSet v _ => singleton_set v
-    | _SIf _ s1 s2 => union (modVars s1) (modVars s2)
-    | _SWhile _ body => modVars body
-    | _SSeq s1 s2 => union (modVars s1) (modVars s2)
-    | _SSkip => empty_set
-    | _SCall binds _ _ | _SIO binds _ _ => of_list binds
+    | Imp_.SLoad v _ => singleton_set v
+    | Imp_.SStore _ _ => empty_set
+    | Imp_.SSet v _ => singleton_set v
+    | Imp_.SIf _ s1 s2 => union (modVars s1) (modVars s2)
+    | Imp_.SWhile _ body => modVars body
+    | Imp_.SSeq s1 s2 => union (modVars s1) (modVars s2)
+    | Imp_.SSkip => empty_set
+    | Imp_.SCall binds _ _ | Imp_.SIO binds _ _ => of_list binds
     end.
 
   Ltac set_solver := set_solver_generic constr:(varname).
@@ -548,30 +548,8 @@ Section ImpVars.
           specialize IH' with (1 := H);
           cbn [modVars] in IH';
           ensure_new IH'
-      end.
-
-      Focus 1.
-      forget ((varset.(@singleton_set set_varname varname) x)) as xx.
-      forget ((Imp.varmap_operations_.(@put varmap varname mword) initialS x v)) as y.
-      clear IHfuel.
-      revert env.
-      repeat match goal with H : _ |- _ => clear H end.
-      intros.
-      Set Printing All.
-      repeat match goal with H : _ |- _ => revert H end.
-
-      Goal
-         forall p : ImpParameters,
-  let Imp : ImpInterface p := Imp.Imp p in
-  forall (set_varname : Type) (varset : set set_varname (Imp.varname p)) (initialS : Imp.varmap p)
-    (xx : set_varname) (y : Imp.varmap p)
-    (_ : forall _ : Imp.funname p,
-         option (prod (prod (list (Imp.varname p)) (list (Imp.varname p))) (@Imp.stmt _ Imp))),
-  @only_differ (Imp.varname p) (Imp.mword p) (Imp.varmap p) (@Imp.varmap_operations_ p) set_varname varset
-    initialS xx y.
-        intros.
-      congruence.
-
+      end;
+      state_calc.
       (* SCall *)
       refine (only_differ_putmany _ _ _ _ _ _); eassumption.
   Qed.
@@ -613,12 +591,12 @@ Definition _c := 2%Z.
 Definition _isRight := 3%Z.
 
 (* RecordImport Imp (* COQBUG(https://github.com/coq/coq/issues/7808) *) *)
-Local Notation expr := Imp.(_expr).
-Local Notation stmt := Imp.(_stmt).
-Local Notation cont := Imp.(_cont).
-Local Notation interp_expr := Imp.(_interp_expr).
-Local Notation interp_stmt := Imp.(_interp_stmt).
-Local Notation interp_cont := Imp.(_interp_cont).
+Local Notation expr := Imp.(expr).
+Local Notation stmt := Imp.(stmt).
+Local Notation cont := Imp.(cont).
+Local Notation interp_expr := Imp.(interp_expr).
+Local Notation interp_stmt := Imp.(interp_stmt).
+Local Notation interp_cont := Imp.(interp_cont).
 
 Eval cbn in
   (fun op : (RISCVImp.ImpParameters_of_RISCVImpParameters _).(bopname) =>
